src/impl/TLS13.Impl.ConnectionState.Network.fsti
@@ -75,7 +75,7 @@ fn mark_received_alert_failure
   (#st0:erased CS.connection_state)
   requires connection_exactly c st0 **
            Pulse.Lib.Array.PtsTo.pts_to raw 'raw_bytes **
-           pure (Ghost.reveal alert <> T.CloseNotify /\
+           pure (Ghost.reveal alert <> T.Close_notify /\
                  Tags.alert_tag_matches alert_wire (Ghost.reveal alert) /\
                  CS.event_raw_delta_legal
                    st0.CS.cs_model
@@ -105,7 +105,7 @@ fn mark_received_close_notify_for_role
                    st0.CS.cs_model
                    (CS.ConnNetworkEvent {
                      CL.message_direction = CL.Received;
-                     CL.message_value = M.TlsAlert T.CloseNotify;
+                     CL.message_value = M.TlsAlert T.Close_notify;
                    })
                    B.empty
                    (Ghost.reveal 'raw_bytes))
@@ -128,7 +128,7 @@ fn mark_received_close_notify
                   st0.CS.cs_model
                   (CS.ConnNetworkEvent {
                     CL.message_direction = CL.Received;
-                    CL.message_value = M.TlsAlert T.CloseNotify;
+                    CL.message_value = M.TlsAlert T.Close_notify;
                   })
                   B.empty
                   (Ghost.reveal 'raw_bytes))
