src/impl/TLS13.Impl.Driver.PairingNoTailInversion.fst
@@ -1109,13 +1109,13 @@ let lemma_client_application_progress_rank_step
        (match msg.CL.message_value with
         | M.TlsAlert alert ->
           (match alert, model.CS.model_control, msg.CL.message_direction with
-           | T.CloseNotify, CS.ControlApplicationData, CL.Sent ->
+           | T.Close_notify, CS.ControlApplicationData, CL.Sent ->
              assert (client_application_progress_rank model <=
                client_application_progress_rank model' + 1)
-           | T.CloseNotify, CS.ControlApplicationData, CL.Received ->
+           | T.Close_notify, CS.ControlApplicationData, CL.Received ->
              assert (client_application_progress_rank model <=
                client_application_progress_rank model' + 1)
-           | T.CloseNotify, CS.ControlClosing, CL.Received ->
+           | T.Close_notify, CS.ControlClosing, CL.Received ->
              assert (client_application_progress_rank model <=
                client_application_progress_rank model' + 1)
            | _, _, _ ->
