src/spec/TLS13.Wire.Spec.Reveal.Util.fsti
@@ -18,10 +18,11 @@ val content_type_byte: ct:T.content_type -> GTot U8.t
 val lemma_content_type_byte_value:
   ct:T.content_type ->
   Lemma (match ct with
-         | T.ChangeCipherSpec -> U8.v (content_type_byte ct) == 0x14
+         | T.Invalid -> U8.v (content_type_byte ct) == 0x00
+         | T.Change_cipher_spec -> U8.v (content_type_byte ct) == 0x14
          | T.Alert -> U8.v (content_type_byte ct) == 0x15
          | T.Handshake -> U8.v (content_type_byte ct) == 0x16
-         | T.ApplicationData -> U8.v (content_type_byte ct) == 0x17)
+         | T.Application_data -> U8.v (content_type_byte ct) == 0x17)
 
 val serialize_record_header:
   content_type:T.content_type ->
@@ -59,7 +60,7 @@ val lemma_byte_32: unit -> Lemma (byte 32 == 32uy)
 val lemma_byte_0303_lo: unit -> Lemma (byte 0x0303 == 0x03uy)
 
 val lemma_content_type_change_cipher_spec_byte:
-  unit -> Lemma (content_type_byte T.ChangeCipherSpec == 0x14uy)
+  unit -> Lemma (content_type_byte T.Change_cipher_spec == 0x14uy)
 
 val lemma_content_type_alert_byte:
   unit -> Lemma (content_type_byte T.Alert == 0x15uy)
@@ -68,7 +69,7 @@ val lemma_content_type_handshake_byte:
   unit -> Lemma (content_type_byte T.Handshake == 0x16uy)
 
 val lemma_content_type_application_data_byte:
-  unit -> Lemma (content_type_byte T.ApplicationData == 0x17uy)
+  unit -> Lemma (content_type_byte T.Application_data == 0x17uy)
 
 val lemma_u8_reveal:
   n:nat ->
